utils.v
@@ -36,25 +36,6 @@ Fixpoint zip {T : Type} (l : List (List T)) : List T :=
   | h::tl => h ++ (zip tl)
 end.
 
-Definition cropBounded {n : nat} {i : Idx n} :
-  to_nat i < S n.
-Proof.
-  apply le_S. apply BoundedInt.
-Qed.
-
-Definition cropleftBounded {n : nat} {i : Idx n} :
-  S(to_nat i) < S n.
-Proof.
-  apply le_n_S. apply BoundedInt.
-Qed.
-
-Definition crop {T : Type} {n : nat} (f : Idx (S n) -> T) : Idx n -> T :=
-  fun i => f (idx (S n) (to_nat i) cropBounded)
-.
-
-Definition crop_left {T : Type} {n : nat} (f : Idx (S n) -> T) : Idx n -> T :=
-  fun i => f (idx (S n) (S(to_nat i)) cropleftBounded)
-.
 
 Fixpoint buildList {T : Type} (n : nat) : (nat -> T) -> List T :=
   match n with
@@ -67,53 +48,6 @@ Fixpoint rev {T : Type} (l : List T) :=
   | [] => []
   | h :: tl => (rev tl) ++ (h :: [])
 end.
-  
-Definition expandBounded {n : nat} {n' : nat} (H : S n < S (S n')) :
-  n < (S n').
-Proof.
-  apply le_S_n. apply H.
-Qed.
 
-Definition expand_left {T : Type} {n : nat} : (Idx n -> T) -> T -> Idx (S n) -> T :=
-  match n with
-  | 0 => fun f im i => im
-  | S n' => fun f im i =>
-            match i with
-            | idx _ 0 H => im
-            | idx _ (S n'') H => f (idx _ n'' (expandBounded H))
-            end
-end.
-
-Definition reverse {T : Type} {n : nat} : (Idx n -> T) -> Idx n -> T :=
-  fun f i => f (idx n (n - 1 - to_nat i) reverseBounded).
-
-Definition expand {T : Type} {n : nat} (f :Idx n -> T) (im : T) : Idx (S n) -> T :=
-  (reverse (expand_left (reverse f) im)).
-
-Fixpoint rtake_left {T : Type} {n : nat} (b : nat) (err : T) : (Idx n -> T) -> (Idx b -> T) :=
-  match n,b with
-  | _,0 => fun f i => err
-  | 0, S b => fun f i => err
-  | S n', S b' => fun (f : Idx (S n') -> T) => expand (rtake_left b' err (crop_left f)) (f zero)
-end.
-
-Fixpoint rtake_right {T : Type} {n : nat} (a : nat) (err : T) : (Idx n -> T) -> (Idx (n-a) -> T) :=
-  match n,a with
-  | 0,_ => fun f i => err
-  | S n',0 => fun (f : Idx (S n') -> T) => (f : Idx ((S n') - 0) -> T)
-  | S n', S a' => fun (f : Idx (S n') -> T) => rtake_right a' err (crop f)
-end.
-
-Definition take_left  {T : Type} {n : nat} (b : nat) (err : T) (f : (Idx n -> T)) : (Idx b -> T) :=
-  reverse (rtake_left b err f)
-.
-
-Definition take_right  {T : Type} {n : nat} (a : nat) (err : T) (f : (Idx n -> T)) : (Idx (n-a) -> T) :=
-  reverse (rtake_right a err (reverse f))
-.
-
-Definition shift {T : Type} {n : nat} {a : nat} {b : nat} (err : T) : (Idx n -> T) -> (Idx (b-a) -> T) :=
-  fun f => take_right a err (take_left b err f)
-.
 
 
